introduced intro method for full state pred using forallsessions

examples/invariants/DY.Example.Invariants.Uniqueness.fst
@@ -2,7 +2,8 @@ module DY.Example.Invariants.Uniqueness
 
 open Comparse
 open DY.Core
-module L = DY.Lib
+module L = DY.Core.Label
+module Lib = DY.Lib
 module List = FStar.List.Tot.Base
 module Trace = DY.Core.Trace.Type
 
@@ -73,33 +74,104 @@ let p_cinvs = {
  preds = default_crypto_predicates default_crypto_usages
 }
 
+noeq type state_predicate_forall_sessions (cinvs:crypto_invariants) = {
+pred: trace -> principal -> state_id -> state_raw -> prop;
+  session_pred: trace -> session_raw -> principal -> state_id -> state_raw -> prop; 
 
+/// the idea for the new full_state_pred:
+/// often the full_state_pred is of the form:
+/// forall_sessions full_st
+/// (fun sid_i sess_i ->
+///    if sid_i = sid
+///    then True // this is a redirect to the session_pred 
+///    else
+///      match sess_i with
+///      | Nil -> True // this is a redirect to the session_pred
+///      | Snoc _ last_i -> pred_on last_i and cont
+/// )
+/// to simplify this, we introduce a new full_state_predicate
+/// that hides this form.
+/// That is, when writing such a full_state_pred we can already assume
+/// that sid_i <> sid and Snoc? sess_i
+  full_state_pred: trace -> sid_i:state_id -> sess_i:session_raw{Snoc? sess_i} -> principal -> sid:state_id{sid_i <> sid} -> state_raw -> prop;
 
-let p_state_pred: state_predicate p_cinvs = {
+  pred_knowable:
+    tr:trace ->
+    prin:principal -> sess_id:state_id -> content:state_raw ->
+    Lemma
+    (requires pred tr prin sess_id content)
+    (ensures
+      is_knowable_by #cinvs (L.principal_state_label prin sess_id) tr content
+    )
+  ;  
+  pred_later:
+    tr1:trace -> tr2:trace ->
+    prin:principal -> sess_id:state_id -> content:state_raw ->
+    Lemma
+    (requires tr1 <$ tr2 /\ pred tr1 prin sess_id content)
+    (ensures pred tr2 prin sess_id content)
+  ;
+  session_pred_grows: 
+    tr1:trace -> tr2:trace -> 
+    sess:session_raw -> prin:principal -> sess_id:state_id -> content:state_raw ->
+    Lemma
+      (requires
+        tr1 <$ tr2 /\ session_pred tr1 sess prin sess_id content
+      )
+      (ensures
+        session_pred tr2 sess prin sess_id content
+      )
+}
+
+/// translating the new full_state_pred to the more general one
+/// implementing the structure from above
+val f : {|cinvs: crypto_invariants |} -> state_predicate_forall_sessions cinvs -> state_predicate cinvs
+let f #cinvs sp = {
+  pred = sp.pred;
+  session_pred = sp.session_pred;
+  full_state_pred = (fun tr full_st p sid cont ->
+    forall_sessions full_st
+    (fun sid_i sess_i -> 
+      if sid_i = sid || Nil? sess_i
+      then True
+      else sp.full_state_pred tr sid_i sess_i p sid cont
+    )
+  );
+  pred_knowable = sp.pred_knowable;
+  pred_later = sp.pred_later;
+  session_pred_grows = sp.session_pred_grows
+}
+ 
+
+let p_state_pred: state_predicate_forall_sessions p_cinvs = {
     pred = (fun tr p sid cont -> is_knowable_by #p_cinvs (principal_state_label p sid) tr cont)
   ; session_pred = (fun tr sess prin sid cont ->
-     True
+     // within a session the idn should stay the same
+     match parse p_state cont with
+     | None -> False
+     | Some (S the_idn _) -> (
+         match sess with
+         | Nil -> True
+         | Snoc init last -> (
+             match parse p_state last with
+             | None -> True
+             | Some last -> last.idn = the_idn
+           )
+       )
     )
-  ; full_state_pred = (fun tr full_st_b p sid cont -> 
+  ; full_state_pred = (fun tr sid_i sess_i p sid cont -> 
+      // across sessions the idn must be different
       match parse p_state cont with
         | None -> False
-        | Some (S the_idn _) -> begin     
-            forall_sessions full_st_b
-            (fun sid_i sess_i -> 
-              match sess_i with
-              | Nil -> True            
-                     // this should always be true (and we should hide it from the user)
-                     // since this corresponds to [session_pred]
-                     // one could also argue that empty sessions should not appear in the full state 
-              | Snoc init_i last_i -> begin
-                    match parse p_state last_i with
-                    | None -> True
-                    | Some last_i ->
-                        if sid_i = sid // if the new state is added to session sid_i
-                          then last_i.idn = the_idn // the id should stay the same within session sid_i
-                          else last_i.idn <> the_idn // otherwise the id must be different
-                end
-            )
+        | Some (S the_idn _) -> begin
+        // using the new full_state_pred
+        // we can make use of the fact that
+        // sess_i is a Snoc 
+        // and we only talk about sid_i <> sid
+            let Snoc _ last_i = sess_i in
+            match parse p_state last_i with
+            | None -> True
+            | Some last_i -> last_i.idn <> the_idn
         end
     )
   ; pred_later = (fun t1 t2 p sid cont -> ())
@@ -110,12 +182,43 @@ let p_state_pred: state_predicate p_cinvs = {
 instance protocol_invariants_p: protocol_invariants = {
   crypto_invs = p_cinvs;
   trace_invs = {
-    state_pred = p_state_pred;
+    state_pred = f p_state_pred;
     event_pred = (fun tr p sid ev -> True)
   }
 }
 
-#push-options "--fuel 2 --z3rlimit 50 --z3cliopt 'smt.qi.eager_threshold=100'"
+/// since the new full_state_pred is of the special form,
+/// we introduce a convenience function to show such a predicate.
+/// This uses the same structure,
+/// which means that the proof does not need to replicate this structure again.
+///
+/// Whan using this method, one as to show the predicate only
+/// for sid_i <> sid and Snoc? sess_i
+/// without having to write these conditions
+let full_state_pred_forall_session_intro
+  (full_st: full_state_raw) 
+  (sid: state_id)
+  (p: (sid_i:state_id{sid_i <> sid}) -> (sess_i:session_raw{Snoc? sess_i}) -> prop)
+  (pf: (sid_i:state_id{sid_i <> sid}) -> (sess_i:session_raw{Snoc? sess_i /\ (sid_i, sess_i) `List.mem` full_st})
+    -> squash (p sid_i sess_i)
+  )
+  : squash (forall_sessions full_st
+    (fun sid_i sess_i ->
+    if sid_i = sid || Nil? sess_i
+      then True 
+      else p sid_i sess_i
+    )
+    )
+= forall_sessions_intro full_st 
+  (fun sid_i sess_i ->
+     sid_i <> sid /\ Snoc? sess_i ==> p sid_i sess_i 
+  )
+  (fun sid_i sess_i ->
+    introduce (sid_i, sess_i) `List.mem` full_st /\ sid_i <> sid /\ Snoc? sess_i ==> p sid_i sess_i 
+    with _ . pf sid_i sess_i
+  )
+
+#push-options "--fuel 2 --z3rlimit 20 --z3cliopt 'smt.qi.eager_threshold=20'"
 val next_full_state_pred:
   tr:trace -> p:principal -> sid:state_id ->
   Lemma 
@@ -137,75 +240,67 @@ let next_full_state_pred tr p sid =
   let S idn c = Some?.v (parse p_state oldst_b) in
   let msg = M p in
   let (_, tr_after_msg) = send_msg (serialize message msg) tr in
-
-  let next_state = S idn (c+1) in
-  let (_,tr_after_next_state) = set_state p sid (serialize p_state next_state) tr_after_msg in
-
   let full_st_b = access_full_state tr_after_msg p in
-  forall_sessions_intro full_st_b
+
+  // using the new method to proof the full_state_pred
+  full_state_pred_forall_session_intro full_st_b sid
+    // the property p is exactly the full_state_pred 
     (fun sid_i sess_i -> 
-       match sess_i with
-       | Nil -> True
-       | Snoc init_i last_i -> (
-           match parse p_state last_i with
-           | None -> True
-           | Some last_i ->
-               if sid_i = sid 
-                 then last_i.idn = idn
-                 else last_i.idn <> idn
-         )
+       let Snoc init_i last_i = sess_i in 
+       match parse p_state last_i with
+       | None -> True
+       | Some last_i -> last_i.idn <> idn
     )
-    (fun sid_i sess_i _ ->
-       match sess_i with
-       | Nil -> ()
-       | Snoc init_i last_i_b ->
-            match parse p_state last_i_b with
-            | None -> ()
-            | Some last_i -> 
-                get_state_same p sid_i tr tr_after_msg;    
-                full_state_mem_get_session_get_state_forall p tr_after_msg;
-                assert(last_i_b = access_state tr_after_msg p sid_i);
-                if sid_i = sid
-                then assert(last_i = S idn c)
-                else (
-                  let oldst_entry = SetState p sid oldst_b in
-                  let tr_after_oldst = tr `suffix_after_event` oldst_entry in
-                  let last_i_entry = SetState p sid_i last_i_b in
-                  let tr_after_last_i = tr `suffix_after_event` last_i_entry in
+    (fun sid_i sess_i -> 
+      // in the proof we can make use of:
+      // sid_i <> sid
+      // Snoc? sess_i
+      // and (sid_i, sess_i) `List.mem` full_st_b
+       let Snoc _ last_i_b = sess_i in 
+       match parse p_state last_i_b with
+       | None -> ()
+       | Some last_i -> 
+           get_state_same p sid_i tr tr_after_msg;    
+           full_state_mem_get_session_get_state_forall p tr_after_msg;
+           assert(last_i_b = access_state tr_after_msg p sid_i);
+           let oldst_entry = SetState p sid oldst_b in
+           let tr_after_oldst = tr `suffix_after_event` oldst_entry in
+           let last_i_entry = SetState p sid_i last_i_b in
+           let tr_after_last_i = tr `suffix_after_event` last_i_entry in
 
-                  if tr_after_oldst `has_suffix` tr_after_last_i
-                  then ( // last_i after oldst on tr
-                    //admit();
-                    get_state_no_set_state_for_on_suffix_after_event tr p sid;
-                    no_set_state_entry_for_on_suffix tr_after_oldst tr_after_last_i p sid;
-                    assert(no_set_state_entry_for p sid tr_after_last_i);
-                    let tr_before_last_i = tr `prefix_before_event` (SetState p sid_i last_i_b) in
-                    suff_after_before_event_is_suff_at_event tr last_i_entry;
-                    no_set_state_entry_for_concat p sid (Snoc Nil (SetState p sid_i last_i_b)) tr_after_last_i;
-                    get_state_same p sid tr_before_last_i tr;
-                    assert(oldst_b = access_state tr_before_last_i p sid);
-                    assert(global_state_pred tr_before_last_i p sid_i last_i_b);
-                    get_state_appears_in_full_state tr_before_last_i p sid
-                  )
-                  else ( // oldst after last_i on tr
-                    // admit();
-                    suffixes tr tr_after_last_i tr_after_oldst;
-                    assert(tr_after_last_i `has_suffix` tr_after_oldst);
+           if tr_after_oldst `has_suffix` tr_after_last_i
+           then ( // last_i after oldst on tr
+             //admit();
+             get_state_no_set_state_for_on_suffix_after_event tr p sid;
+             no_set_state_entry_for_on_suffix tr_after_oldst tr_after_last_i p sid;
+             assert(no_set_state_entry_for p sid tr_after_last_i);
+             let tr_before_last_i = tr `prefix_before_event` (SetState p sid_i last_i_b) in
+             suff_after_before_event_is_suff_at_event tr last_i_entry;
+             no_set_state_entry_for_concat p sid (Snoc Nil (SetState p sid_i last_i_b)) tr_after_last_i;
+             get_state_same p sid tr_before_last_i tr;
+             assert(oldst_b = access_state tr_before_last_i p sid);
+             assert(global_state_pred tr_before_last_i p sid_i last_i_b);
+             get_state_appears_in_full_state tr_before_last_i p sid
+           )
+           else ( // oldst after last_i on tr
+             //admit();
+             suffixes tr tr_after_last_i tr_after_oldst;
+             assert(tr_after_last_i `has_suffix` tr_after_oldst);
 
-                    get_state_no_set_state_for_on_suffix_after_event tr p sid_i;
-                    no_set_state_entry_for_on_suffix tr_after_last_i tr_after_oldst p sid_i;
-                    let tr_before_old = tr `prefix_before_event` oldst_entry in                               
-                    suff_after_before_event_is_suff_at_event tr oldst_entry;
-                    no_set_state_entry_for_concat p sid_i (Snoc Nil oldst_entry) tr_after_oldst;
-                    get_state_same p sid_i tr_before_old tr;
-                    let state_i_before_old = access_state tr_before_old p sid_i in
-                    assert(state_i_before_old = last_i_b);
-                    assert(global_state_pred tr_before_old p sid oldst_b);
-                    get_state_appears_in_full_state tr_before_old p sid_i  
-                  )
-                )
+             get_state_no_set_state_for_on_suffix_after_event tr p sid_i;
+             no_set_state_entry_for_on_suffix tr_after_last_i tr_after_oldst p sid_i;
+             let tr_before_old = tr `prefix_before_event` oldst_entry in                               
+             suff_after_before_event_is_suff_at_event tr oldst_entry;
+             no_set_state_entry_for_concat p sid_i (Snoc Nil oldst_entry) tr_after_oldst;
+             get_state_same p sid_i tr_before_old tr;
+             let state_i_before_old = access_state tr_before_old p sid_i in
+             assert(state_i_before_old = last_i_b);
+             assert(global_state_pred tr_before_old p sid oldst_b);
+             get_state_appears_in_full_state tr_before_old p sid_i  
+           )
     )
 #pop-options
+
 
 #push-options "--z3rlimit 25"
 val next_invariant: tr:trace -> p:principal -> sid:state_id ->
@@ -234,6 +329,8 @@ let next_invariant tr p sid =
           serialize_wf_lemma message (is_publishable tr) msg;
 
           serialize_wf_lemma p_state (is_knowable_by (principal_state_label p sid) tr_after_msg) next_state;
+
+          get_session_same p sid tr tr_after_msg;
 
           next_full_state_pred tr p sid
         )
