src/core/DY.Core.Trace.State.Aux.fst
@@ -33,12 +33,12 @@ let forall_sessions (fst:full_state_raw) (p:state_id -> session_raw ->  prop)  :
 let forall_sessions_intro 
   (full_st: full_state_raw)
   (p: state_id -> session_raw -> prop)
-  (pf: ( (sid:state_id) -> (sess:session_raw) -> squash ((sid,sess) `List.mem` full_st) -> Tot (squash ( p sid sess)) ))
+  (pf: ( (sid:state_id) -> (sess:session_raw{(sid,sess) `List.mem` full_st}) -> Tot (squash ( p sid sess)) ))
   : (squash ( forall_sessions full_st p ))
 = introduce forall sid sess. (sid, sess) `List.mem` full_st ==> p sid sess 
   with  
     introduce (sid, sess) `List.mem` full_st ==> p sid sess 
-    with _ . pf sid sess _
+    with _ . pf sid sess 
     
 
 val max: nat -> nat -> nat
